code/experimental/P256/Hacl.Impl.P256.fsti
@@ -118,6 +118,20 @@ val point_add: p: point -> q: point -> result: point -> tempBuffer: lbuffer uint
   )
 
 
+val isPointAtInfinityPrivate: p: point -> Stack uint64
+  (requires fun h -> live h p)
+  (ensures fun h0 r h1 -> modifies0 h0 h1 /\          
+    (
+      (uint_v r == 0 \/ uint_v r == maxint U64) /\ 
+      (
+	let x = as_nat h0 (gsub p (size 0) (size 4)) in 
+	let y = as_nat h0 (gsub p (size 4) (size 4)) in 
+	let z = as_nat h0 (gsub p (size 8) (size 4)) in 
+	let rr =  Hacl.Spec.P256.isPointAtInfinity (x, y, z) in 
+	if uint_v r = 0 then rr = false else rr = true))
+    )
+
+
 val norm: p: point -> resultPoint: point -> tempBuffer: lbuffer uint64 (size 88) -> Stack unit
   (requires fun h -> live h p /\ live h resultPoint /\ live h tempBuffer /\ disjoint p tempBuffer /\ disjoint tempBuffer resultPoint /\ 
     as_nat h (gsub p (size 0) (size 4)) < prime /\
@@ -140,17 +154,6 @@ val norm: p: point -> resultPoint: point -> tempBuffer: lbuffer uint64 (size 88)
       z3 == 1 
    )   
   )
-
-
-val isPointAtInfinityPrivate: p: point -> Stack uint64
-  (requires fun h -> live h p)
-  (ensures fun h0 r h1 -> modifies0 h0 h1 /\          
-    (
-      let x = as_nat h0 (gsub p (size 0) (size 4)) in 
-      let y = as_nat h0 (gsub p (size 4) (size 4)) in 
-      let z = as_nat h0 (gsub p (size 8) (size 4)) in 
-      let rr =  Hacl.Spec.P256.isPointAtInfinity (x, y, z) in 
-      if uint_v r = 0 then rr = true else rr = false))
 
 
 
